#import "lecture-template.typ": *

#set document(
  title: "MATH 108A Notes Jan. 29, 2026",
  date: datetime(day: 29, month: 1, year: 2026),
)

#show: template

#theorem(number: none)[
  Let $S = { v_1, v_2, ..., v_n }$ be a linearly independent subset of a vector space $V(FF)$, and suppose $v in V$ where $v$ is also a vector in $S$.

  Then $S union { v }$ is linearly dependent if and only if $v in span(S)$.
]

#proof[
  Suppose $S union { v }$ is linearly dependent. Then there is some nonzero constant $c$ for which

  $
        & c_1 v_1 + c_2 v_2 + dots.c + c_n v_n + c v && = bold(0) \
    ==> & c_1 v_1 + c_2 v_2 + dots.c + c_n v_n       && = - c v wide c_i in FF thick forall i in [n].
  $

  Then, since $c != 0$, we multiply both sides by $c^(-1)$ to get

  $
    v = c^(-1)(c_1 v_1 + c_2 v_2 + dots.c + c_n v_n).
  $

  Thus, $v in span(S)$.

  Conversely, suppose $v in span(S)$. Then $v$ can be expressed as a linear combination of vectors in $S$, like so:

  $
    v = c_1 v_1 + c_2 v_2 + dots.c + c_n v_n wide c_i in FF thick forall i in [n].
  $

  Adding $-v$ to both sides, we obtain

  $
    bold(0) = -1v + c_1 v_1 + c_2 v_2 + dots.c + c_n v_n.
  $

  Thus, there exists a nontrivial combination of vectors in $S union { v }$ that equals the zero vector. By definition, this set is linearly dependent.
]

#theorem(number: none)[
  Let $S = { v_i }_(i = 1)^n$ be a linearly dependent subset of a vector space $V(FF)$. Then there exists some index $k in [n]$ for which

  $
    v_k in span{ v_1, v_2, ..., v_(k - 1) }.
  $

  Furthermore, $span(S) = span(S without { v_k })$.
]

#proof[
  Given that $S = { v_1, ..., v_n }$ is linearly dependent, there are some $c_i in FF$, not all zero, such that

  $
    c_1 v_1 + c_2 v_2 + dots.c + c_n v_n = bold(0).
  $

  Choose $k in [n]$ to be the largest number for which $c_k != 0$. We then have

  $
    c_1 v_1 + dots.c + c_k v_k + dots.c + c_n v_n = bold(0).
  $

  Adding $-c_k v_k$ to both sides and multiplying by $c_k^(-1)$, we get

  $
    v_k & = c_k^(-1)(c_1 v_1 + dots.c + c_(k - 1) v_(k - 1) + 0v_k + 0v_(k + 1) + dots.c + 0v_n) \
        & = c_k^(-1)(c_1 v_1 + dots.c + c_(k - 1) v_(k - 1)).
  $

  Therefore, $v_k in span { v_1, v_2, ..., v_(k - 1) }$.

  We now show that $span(S) = span(S without { v_k })$. Let $v in span(S without { v_k })$. Then

  $
    v &= limits(sum)_(i = 1)^(k - 1) c_i v_i + limits(sum)_(i = k + 1)^n c_i v_i \
    &= limits(sum)_(i = 1)^(k - 1) c_i v_i + 0v_k + limits(sum)_(i = k + 1)^n c_i v_i wide v_i in S, c_i in FF thick forall i in [n].
  $

  Thus, $v in span(S)$, which implies $span(S without { v_k}) subset.eq span(S)$.

  Conversely, let $v in span(S)$. Then

  $
    v = limits(sum)_(i = 1)^n c_i v_i = limits(sum)_(i = 1)^(k - 1) c_i v_i + c_k v_k + limits(sum)_(i = k + 1)^n c_i v_i wide v_i in S, c_i in FF thick forall i in [n].
  $

  We know that $v_k$, and thereby $c_k v_k$, exist in $span{ v_1, v_2, ..., v_(k - 1)}$. This implies

  $
    c_k v_k = d_1 v_1 + d_2 v_2 + dots.c + d_(k - 1) v_(k - 1) wide d_i in FF thick forall i in[n].
  $

  Substituting this expression back into the expansion of $v$, we get

  $
    v = limits(sum)_(i = 1)^(k - 1) (c_i + d_i) v_i + limits(sum)_(i = k + 1)^n c_i v_i.
  $

  Thus, $v$ can be written as a linear combination of vectors in $S without { v_k }$. This implies $v in span(S without { v_k })$, meaning $span(S) subset.eq span(S without { v_k })$.

  It follows that $span(S) = span(S without { v_k })$.
]

#remark[
  This theorem tells us that deleting a vector from a linearly dependent set does not change its span.
]

#theorem(number: none)[The Replacement Theorem][
  Let $V(FF)$ be a vector space generated by a finite set $S$ for which $abs(S) = n < oo$. Furthermore, let $L$ be a linearly independent subset of $V$ for which $abs(L) = m < oo$.

  + $m <= n$, and $abs(S) <= |L|$.

  + There is a subset $H subset.eq S$ containing exactly $n - m$ vectors such that $L union H$ generates $V$.
]

#pagebreak()

#proof[
  Let $S = { x_i }_(i = 1)^n subset.eq V(FF)$ such that $span(S) = V$. We proceed by mathematical induction on $m$.

  If $m = 0$, then $m <= n$ for every natural number $n$. Moreover, $m = 0$ implies $L$ is the empty set, so taking $H = S$ gives the desired result.

  Now, assume that the result holds for some integer $m > 0$. We show that the result also holds for $m + 1$.

  Let $L = { v_1, v_2, ..., v_(m + 1) }$ be a linearly independent subset of $V$ containing $m + 1$ elements. By a previous result, any finite subset of a linearly independent set is also linearly independent. Thus, the set ${ v_1, v_2, ..., v_m } subset.eq L$  is linearly independent.

  By the inductive hypothesis, $m <= n$, and there exists a subset ${ x_1, x_2, ..., x_(n - m) } subset.eq S$ such that ${ v_1, v_2, ..., v_m } union { x_1, x_2, ..., x_(n - m) }$ generates $V$.

  Now, we know $v_(m + 1) in V$, so it can be written as a linear combination of vectors in the above union. That is,

  $
    v_(m + 1) = c_1 v_1 + dots.c + c_m v_m + d_1 x_1 + dots.c + d_(n - m) x_(n - m) \ c_i in FF thick forall i in [m], quad d_i in FF thick forall i in [n - m].
  $

  Note that $n - m > 0$, since otherwise $n - m = 0$ would imply $v_(m + 1)$ is a linear combination of vectors in ${ v_1, v_2, ..., v_(m + 1) } subset.eq L$. That would be a contradiction, since $L$ is linearly independent. Thus, $n > m$, and $n >= m + 1$.

  Moreover, some $d_i$ must be nonzero, otherwise we would reach the same contradiction. Take $d_1 != 0$. From our expansion of $v_(m + 1)$, we get

  $
    x_1 = -d_1^(-1) (c_1 v_1 + dots.c + c_m v_m + d_2 x_2 + d_(n - m) x_(n - m) - v_(m + 1)).
  $

  Let $H = { x_2, x_3, ..., x_(n - m) }$. Note that $abs(H) = n - m - 1 = n - (m + 1)$. Then $x_1$ is a linear combination of vectors in $L$ and $H$. In other words, $x_1 in span(L union H)$.

  All vectors $v_1, ..., v_m$ exist in $L$, so they are also elements of $span(L union H)$. Similarly, since $x_2, ..., x_(n - m)$ are all in $H$, they are vectors in $span(L union H)$. We just showed that $x_1 in span(L union H)$. These facts combined give ${ v_1, ..., v_m, x_1, ..., x_(n - m)} subset.eq span(L union H)$.

  It follows that $span { v_1, ..., v_m, x_1, ..., x_(n - m) } subset.eq span(L union H)$. However, we also know the set ${ v_1, ..., v_m, x_1, ..., x_(n - m) }$ generates $V$. Therefore, $span(L union H) = V$. The conclusion then holds for $m + 1$.
]

#definition(number: none)[Basis for a Vector Space][
  A *basis* for a vector space $V(FF)$ is a linearly independent subset of $V$ that generates $V$. We usually represent bases with the symbol $beta$.
]

#example[
  The set ${ (1, 2), (3, 5) }$ is a basis for $RR^2$.
]

#example[
  The basis for the zero vector space ${ bold(0) }$ is the empty set.
]

#example[
  One basis for $FF^n$ is a set of $n$-tuples

  $
    { (1, 0, ..., 0), (0, 1, ..., 0), ..., (0, ..., 0, 1) } = { e_1, e_2, ..., e_n }.
  $

  This is the *standard basis* for $FF^n$.
]
